prove first SimplifyCFG round evaluation

lowering/defs/evalCompilerBytecodeSimplifyCfgProbeScript.sml
@@ -273,4 +273,163 @@ Theorem first_simplify_cfg_substituted_entry:
 Proof
   ACCEPT_TAC first_substituted_entry_th
 QED
+
+fun eval_first_substituted_reachable bb =
+  let
+    val label_th =
+      computeLib.EVAL_CONV (mk_comb (``\bb : basic_block. bb.bb_label``, bb))
+    val reachable_tm =
+      list_mk_comb (``reachable``,
+        [``first_simplify_cfg_substituted``, rhs (concl label_th)])
+  in
+    computeLib.EVAL_CONV reachable_tm
+  end
+
+val first_substituted_reachable_ths =
+  map eval_first_substituted_reachable first_substituted_blocks
+val first_final_remove_th =
+  SIMP_CONV (srw_ss ())
+    (simplifyCfgDefsTheory.remove_unreachable_blocks_def ::
+     first_simplify_cfg_substituted_entry ::
+     first_simplify_cfg_substituted_blocks ::
+     first_substituted_reachable_ths)
+    ``remove_unreachable_blocks first_simplify_cfg_substituted``
+val first_final_removed_tm = rhs (concl first_final_remove_th)
+
+Definition first_simplify_cfg_final_removed_def:
+  first_simplify_cfg_final_removed = ^first_final_removed_tm
+End
+
+Theorem exact_first_final_remove_unreachable:
+  remove_unreachable_blocks first_simplify_cfg_substituted =
+    first_simplify_cfg_final_removed
+Proof
+  simp[first_simplify_cfg_final_removed_def] >>
+  ACCEPT_TAC first_final_remove_th
+QED
+
+Theorem first_simplify_cfg_substituted_dispatch_edge:
+  ~fn_succ first_simplify_cfg_substituted "__entry" "@dispatch_1"
+Proof
+  simp[cfgTransformTheory.fn_succ_def,
+       venomInstTheory.lookup_block_def, venomInstTheory.bb_succs_def,
+       venomInstTheory.get_successors_def, venomInstTheory.is_terminator_def,
+       venomStateTheory.get_label_def, listTheory.FIND_def,
+       listTheory.INDEX_FIND_def, first_simplify_cfg_substituted_def]
+QED
+
+Theorem first_simplify_cfg_substituted_fallback_edge:
+  ~fn_succ first_simplify_cfg_substituted "__entry" "@fallback_0"
+Proof
+  simp[cfgTransformTheory.fn_succ_def,
+       venomInstTheory.lookup_block_def, venomInstTheory.bb_succs_def,
+       venomInstTheory.get_successors_def, venomInstTheory.is_terminator_def,
+       venomStateTheory.get_label_def, listTheory.FIND_def,
+       listTheory.INDEX_FIND_def, first_simplify_cfg_substituted_def]
+QED
+
+Theorem first_simplify_cfg_substituted_no_entry_succ:
+  !lbl. ~fn_succ first_simplify_cfg_substituted "__entry" lbl
+Proof
+  simp[cfgTransformTheory.fn_succ_def,
+       venomInstTheory.lookup_block_def, venomInstTheory.bb_succs_def,
+       venomInstTheory.get_successors_def, venomInstTheory.is_terminator_def,
+       venomStateTheory.get_label_def, listTheory.FIND_def,
+       listTheory.INDEX_FIND_def, first_simplify_cfg_substituted_def]
+QED
+
+Theorem first_simplify_cfg_substituted_dispatch_unreachable:
+  ~RTC (fn_succ first_simplify_cfg_substituted) "__entry" "@dispatch_1"
+Proof
+  simp[Once relationTheory.RTC_CASES1,
+       first_simplify_cfg_substituted_no_entry_succ]
+QED
+
+Theorem first_simplify_cfg_substituted_fallback_unreachable:
+  ~RTC (fn_succ first_simplify_cfg_substituted) "__entry" "@fallback_0"
+Proof
+  simp[Once relationTheory.RTC_CASES1,
+       first_simplify_cfg_substituted_no_entry_succ]
+QED
+
+val first_final_literal_reach_ths =
+  map (REWRITE_RULE [first_simplify_cfg_substituted_def])
+    [first_simplify_cfg_substituted_dispatch_unreachable,
+     first_simplify_cfg_substituted_fallback_unreachable]
+val first_final_removed_normal_eq =
+  SIMP_RULE (srw_ss ()) first_final_literal_reach_ths
+    first_simplify_cfg_final_removed_def
+val first_final_removed_blocks_th =
+  SIMP_RULE (srw_ss ()) []
+    (AP_TERM ``\fn : ir_function. fn.fn_blocks``
+      first_final_removed_normal_eq)
+val first_final_removed_blocks =
+  fst (listSyntax.dest_list (rhs (concl first_final_removed_blocks_th)))
+
+Theorem first_simplify_cfg_final_removed_blocks:
+  ^(concl first_final_removed_blocks_th)
+Proof
+  ACCEPT_TAC first_final_removed_blocks_th
+QED
+
+fun eval_first_final_phi_repair bb =
+  let
+    val label_th =
+      computeLib.EVAL_CONV (mk_comb (``\bb : basic_block. bb.bb_label``, bb))
+    val label_tm = rhs (concl label_th)
+    val preds_tm =
+      list_mk_comb (``pred_labels``,
+        [``first_simplify_cfg_final_removed``, label_tm])
+    val preds_th =
+      SIMP_CONV (srw_ss ())
+        [first_final_removed_normal_eq,
+         cfgTransformTheory.pred_labels_def,
+         cfgTransformTheory.block_preds_def,
+         venomInstTheory.bb_succs_def,
+         venomInstTheory.get_successors_def,
+         venomInstTheory.is_terminator_def,
+         venomStateTheory.get_label_def]
+        preds_tm
+    val repair_tm =
+      list_mk_comb (``fix_phis_in_block``, [rhs (concl preds_th), bb])
+    val repair_th = computeLib.EVAL_CONV repair_tm
+  in
+    [preds_th, repair_th]
+  end
+
+val first_final_phi_repair_ths =
+  List.concat (map eval_first_final_phi_repair first_final_removed_blocks)
+val first_final_fix_all_phis_th =
+  SIMP_CONV (srw_ss ())
+    (simplifyCfgDefsTheory.fix_all_phis_def ::
+     first_simplify_cfg_final_removed_blocks :: first_final_phi_repair_ths)
+    ``fix_all_phis first_simplify_cfg_final_removed``
+val first_round1_fn_tm = rhs (concl first_final_fix_all_phis_th)
+
+Definition first_simplify_cfg_round1_fn_def:
+  first_simplify_cfg_round1_fn = ^first_round1_fn_tm
+End
+
+Theorem exact_first_final_fix_all_phis:
+  fix_all_phis first_simplify_cfg_final_removed =
+    first_simplify_cfg_round1_fn
+Proof
+  simp[first_simplify_cfg_round1_fn_def] >>
+  ACCEPT_TAC first_final_fix_all_phis_th
+QED
+
+Theorem exact_first_simplify_cfg_round_with_labels:
+  simplify_cfg_round_with_labels first_simplify_cfg_operand =
+    (first_simplify_cfg_round1_fn, REVERSE ^first_collapse_label_map_tm)
+Proof
+  simp[simplifyCfgDefsTheory.simplify_cfg_round_with_labels_def,
+       first_simplify_cfg_operand_entry,
+       exact_first_remove_unreachable_named,
+       exact_first_fix_all_phis,
+       exact_first_collapse_dfs_components,
+       exact_first_substitution,
+       exact_first_final_remove_unreachable,
+       exact_first_final_fix_all_phis]
+QED
+
 val _ = export_theory()
